\documentclass[a4paper,12pt]{article}
\usepackage[a4paper, hmargin={3cm,2cm}, vmargin={2cm,2cm}]{geometry}
\usepackage{amsmath}
\usepackage{amsthm}
\usepackage{amsfonts}
\usepackage{color}
\usepackage[final]{graphicx}
\usepackage{subcaption}
\usepackage{wrapfig}
\newtheorem{remark}{Remark}[]
\newtheorem{prop}{Proposition}
\usepackage{amssymb}

\newcommand{\R}{\mathbb{R}}
\newcommand{\C}{\mathbb{C}}
\newcommand{\N}{\mathbb{N}}
\newcommand{\Q}{\mathbb{Q}}
\newcommand{\W}{\mathbb{W}}
\newcommand{\Vspace}{\mathbb{V}}
\newcommand{\Hspace}{\mathbb{H}}
\newcommand{\Lspace}{\mathbb{L}}
\newcommand{\Lagr}{\mathcal{L}}


% Title Page
\title{Seminar Notes Alifian}
\author{Alifian Mahardhika Maulana}


\begin{document}
\maketitle
\section{3D Linear Elasticity}
\begin{equation}\nonumber
\begin{aligned}
\Omega \subset \R^d & (d=2,3) \\
u = \Omega & \rightarrow \R^2 \text{(small displacement)}\\
x & \mapsto u(x)
\end{aligned}
\end{equation}
\subsection{Strain Tensor}
\begin{equation}
\begin{aligned}
e[u] & = (e_{ij}[u]) \in \R^{d x d}_{sym}\\
e[u] & := \frac{1}{2} (\bigtriangledown^Tu + (\bigtriangledown^Tu)^T)
\end{aligned}
\end{equation}
\subsection{Stress Tensor}
\begin{equation}
\begin{aligned}
\sigma[u] &= (\sigma{ij}[u]) \in \R^{d x d}_{sym}\\
\end{aligned}
\end{equation}
Based on Hook's Law, stress tensor must have equality with strain so that
\begin{equation}\nonumber
\begin{aligned}
\sigma &= \textbf{C} e\\
\text{with } \textbf{C} &= \textbf{C}_{ijkl} \text{(is a 4th order elasticity tensor)}\\
\sigma{ij} &= \textbf{C}{ijkl} e_{kl}\\
\textbf{C}_{ijkl} &= \textbf{C}_{ijlk} = \textbf{C}_{klij} \text{(symmetry)}\\
\textbf{C}_{ijkl} \xi_{ij} \xi_{kl} & \geq \textbf{C}_* |\xi|^2
\end{aligned}
\end{equation}
\subsection{Boundary Value Problem}
\begin{equation}
\begin{cases}
-\partial_i \sigma_{ij}[u] &= f_j(x), x \in \Omega\\
u &= g(x), x \in \Gamma_D\\
\sigma[u]_\nu &= q(x), x \in \Gamma_N
\end{cases}
\end{equation}
\newpage
\subsection{Equilibrium Equations of Force in $\Omega$ and on $\Gamma_N$}
\subsubsection{Strain Energy Density}
\begin{equation}
\label{energy_density}
\omega[u](x) := \frac{1}{2} \sigma[u] : e[u]
\end{equation}
Solving using Sobolev Space in Isotropic Case, equation \ref{energy_density} becomes
\begin{equation}\nonumber
c_{ijkl} = \lambda \delta_{ij} \delta_{kl} + \mu(\delta_{ik} \delta_{jl} + \delta_{il} \delta_{jk})
\end{equation}
with $\lambda, \mu$ called Lame Constant
\begin{equation}\nonumber
\delta_{ij} = \begin{cases}
1, i = j\\
0, i \neq j
\end{cases}
\end{equation}
\begin{equation}\nonumber
\begin{aligned}
\sigma[u] &= (\sigma_{ij}[u])\\
\sigma_{ij}[u] &= c_{ijkl} e_{kl}[u]\\
&= \lambda(\delta_k u_k)\delta_{ij} + \mu(\delta_i u_j + \delta_j u_i)\\
&= \lambda(\text{div } u) I + 2\mu e[u]
\end{aligned}
\end{equation}
\begin{equation}\nonumber
\begin{aligned}
\omega[u] = \frac{1}{2} (\lambda(\text{div } u) I + 2\mu e[u]) : e[u]\\
\omega[u] = \frac{1}{2} (\lambda(\text{div } u)^2 + \mu |e[u]|^2\\
\end{aligned}
\end{equation}
\begin{remark}
Positivity of \textbf{C}
\begin{equation}\nonumber
\begin{aligned}
(\textbf{C} \xi) : \xi \geq \textbf{C}_* |\xi|^2 (\forall \xi \in \R^{d x d}_{sym})\\
(\textbf{C} \xi) : \xi = \lambda |\text{tr }\xi|^2 + 2\mu|\xi|^2\\
\end{aligned}
\end{equation}
If $\lambda \geq 0, \mu > 0$, then $C_* = 2 \mu$
\begin{equation}\nonumber
\xi = (\xi_{ij}), |\xi|^2 = \xi_{ij} \xi_{ij} = \sum_{i = 1 \dots d}^{d} \sum_{j = 1 \dots d}^{d} |\xi_{ij}|^2
\end{equation}
\end{remark}
\subsection{Elasticity Problem}
\begin{equation}
\begin{cases}
-\text{div } \sigma[u] &= f(x) \text{ in } \Omega \subset \R^d\\
u &= g(x) \text{ on } \Gamma_D\\
\sigma[u]v &= q(x) \text{ on } \Gamma_N
\end{cases}
\end{equation}
\subsection{Crack Problem}
\begin{equation}
\begin{cases}
-\text{div } \sigma[u] &= f(x) \text{ in } \Omega \setminus \Sigma \subset \R^d\\
u &= g(x) \text{ on } \Gamma_D\\
\sigma[u]v &= q(x) \text{ on } \Gamma_N\\
\sigma[u]v &= 0 \text{ on } \Sigma^+ \cup \Sigma^-
\end{cases}
\end{equation}
\subsection{Lebesque Measurable Theory}
\begin{equation}
L^p(\Omega) := \Bigg\{v:\Omega \rightarrow \R|\begin{cases}
v = \text{Lebesque measurable}\\
\int_\Omega|v(x)|^p dx < \infty
\end{cases}\Bigg\}
\end{equation}
\begin{remark}
	for $u,v \in \Lspace^p(\Omega), \text{ if } \exists N \subset \Omega$
	such that $\begin{cases}
		u(x) = v(x) (x \in \Omega \setminus \text{N})\\
		\Lagr^d(N) = 0,
	\end{cases}$
	then we identify $u$ and $v$,
	$\Lagr^d(N) = 0 \Leftrightarrow \text{volume of N } = 0$
	for simplicity, we also can say that
	$u(x) = v(x) \text{ for a.e. } x \in \Omega$
\end{remark}
for example
\begin{equation}
\begin{aligned}
&v:\R \rightarrow \R\\
&v(x) = \begin{cases}
1, x \in \Q\\
0, x \in \R \setminus \Q\\
\end{cases}\\
&\int_\R v dx = 0, \Lagr^1(\Q) = 0\\
&v(x) = 0 \text{ on } \R \setminus \Q, \text{ or we can say } v = 0 \text{ a.e. in } \R
\end{aligned}
\end{equation}
\subsection{Sobolev Space}
\begin{equation}
\W^{1,p}(\Omega) := \bigg\{v\in\Lspace^p(\Omega)\frac{\partial v}{\partial x_j}_{(j=1\dots d)}\in\Lspace^p(\Omega)\bigg\}
\end{equation}
such $\frac{\partial v}{\partial x_j}$ we called it distribution sence.\\
example of Sobolev Space is as follow:
\begin{equation}\nonumber
v \in \Lspace^p(\Omega) \text{ if } \exists \omega_j \in \Lspace(\Omega)
\end{equation}
such that
\begin{equation}\nonumber
\begin{aligned}
\int_\Omega v \frac{\partial \varphi}{\partial x_j} dx = -\int_\Omega \omega_j \varphi dx (\forall \varphi \in \C_0^\infty(\Omega))\\
\Rightarrow \frac{\partial \varphi}{\partial x_j} = \omega_j \text{ in distribution sence}
\end{aligned}
\end{equation}
for
\begin{equation}\nonumber
\begin{aligned}
v \in \C^1(\Omega), &\frac{\partial v}{\partial x_j} (x) = \omega_j(x)\\
&\Updownarrow\\
\int_\Omega \omega_j \varphi dx &= -\int_\Omega v \frac{\partial \varphi}{\partial x_j}dx (\forall \varphi \in \C_0^\infty(\Omega))
\end{aligned}
\end{equation}
In particular,
\begin{equation}\nonumber
\Hspace^1(\Omega) := \W^{1,2}(\Omega), \bigtriangledown u = \left(\begin{array}{c}
\frac{\partial u}{\partial x_1}\\
\vdots\\
\frac{\partial u}{\partial x_d}
\end{array}\right)
\end{equation}
inner product
\begin{equation}\nonumber
(u,v)_{\Hspace^1(\Omega)} := \int_\Omega uv\ dx + \int_\Omega \bigtriangledown u \cdot \bigtriangledown v\ dx
\end{equation}
norm
\begin{equation}\nonumber
||u||_{\Hspace^1(\Omega)} := \sqrt{(u,v)_{\Hspace^1(\Omega)}} = \sqrt{\int_\Omega|u|^2dx + \int_\Omega|\bigtriangledown u|^2dx}
\end{equation}
$\Hspace^1(\Omega)$ is complete ($\Hspace^1(\Omega)$ is a Hilbert Space)
\begin{equation}\nonumber
(u,v)_{\Lspace^2(\Omega)} = \int_\Omega uv dx
\end{equation}
\subsection{Incomplete Hilbert Space}
$\Vspace : \text{ a vector space in } \R$
\begin{equation}\nonumber
\begin{aligned}
\begin{cases}
u,v\ \in \Vspace \Rightarrow \alpha u + \beta v \in \Vspace\\
\alpha,\beta\ \in \R
\end{cases}
\end{aligned}
\end{equation}
$\text{If } (\cdot,\cdot) : \Vspace \times \Vspace \rightarrow \R \text{ satisfies}$
\begin{equation}\nonumber
\begin{aligned}
\begin{cases}
(u\cdot v) \geq 0 \text{ and } (u,u) = 0 \Leftrightarrow u = 0_v \in \Vspace\\
(u,v) = (v,u)\\
(\alpha u + \beta v, \omega) = \alpha(u,\omega) + \beta (v,\omega)
\end{cases}
\end{aligned}
\end{equation}
then we call $[\Vspace \times \Vspace]$ pre Hilbert space or incomplete Hilbert Space.
\subsection{Property of $\Lspace^2(\Omega)$}
For $v \in \C^1(\Omega),$
\begin{equation}\nonumber
\begin{aligned}
\frac{\partial v}{\partial x_j}(x)&=w_j(x)\\
&\Updownarrow\\
\int_\Omega w_j\varphi dx &= -\int\Omega v \frac{\partial \varphi}{\partial x_j} dx\ \big(\forall\varphi\in\C_0^\infty(\Omega)\big)\\
\end{aligned}
\end{equation}
$(u,v)_{\Lspace^2(\Omega)} = \int_\Omega uv dx\\$
\begin{equation}\nonumber
\Rightarrow \bigg|\int_{\Omega}uvdx\bigg| \leq \int_{\Omega}|u||v|dx \leq ||u||_{\Lspace^2(\Omega)} ||v||_{\Lspace^2(\Omega)}
\end{equation}
$u,v \in \Hspace^1(\Omega)$
\begin{equation}\nonumber
\begin{aligned}
\Rightarrow \frac{\partial u}{\partial x_j}, \frac{\partial v}{\partial x_j} & \in {\Lspace^2(\Omega)}\\
\bigg| \int_\Omega \frac{\partial u}{\partial x_j} \frac{\partial v}{\partial x_j}dx\bigg| \leq \int_\Omega \bigg| \frac{\partial u}{\partial x_j} \bigg| \bigg| \frac{\partial v}{\partial x_j} \bigg| dx & \leq \bigg|\bigg| \frac{\partial u}{\partial x_j}\bigg|\bigg|_{\Lspace^2(\Omega)} \bigg|\bigg| \frac{\partial v}{\partial x_j} \bigg|\bigg|_{\Lspace^2(\Omega)}\\
\triangledown u \cdot \triangledown v &= \sum_{j=1}^{d}\frac{\partial u}{\partial x_j} \frac{\partial v}{\partial x_j}\\
\bigg| \int_{\Omega} \triangledown u \cdot \triangledown v dx \bigg| &= \bigg| \int \sum_{j=1}^{d}\frac{\partial u}{\partial x_j} \frac{\partial v}{\partial x_j} dx \bigg| \leq  \sum_{j=1}^{d} \int \bigg| \frac{\partial u}{\partial x_j} \bigg| \bigg|  \frac{\partial v}{\partial x_j} \bigg| dx\\
&\leq \sum_{j=1}^{d} \bigg|\bigg| \frac{\partial u}{\partial x_j} \bigg|\bigg|_{\Lspace^2(\Omega)} \bigg|\bigg| \frac{\partial v}{\partial x_j} \bigg|\bigg|_{\Lspace^2(\Omega)}\\
&\leq \sqrt{\sum_{j=1}^{d} \bigg|\bigg| \frac{\partial u}{\partial x_j} \bigg|\bigg|_{\Lspace^2(\Omega)}} \sqrt{\sum_{j=1}^{d} \bigg|\bigg| \frac{\partial v}{\partial x_j} \bigg|\bigg|_{\Lspace^2(\Omega)}}\\
&= \sqrt{\sum_{j=1}^{d}\int_\Omega\bigg|\frac{\partial u}{\partial x_j}\bigg|^2 dx} \sqrt{\sum_{j=1}^{d}\int_\Omega\bigg|\frac{\partial v}{\partial x_j}\bigg|^2 dx}\\
&= \sqrt{\int_\Omega\bigg(\sum_{j=1}^{d}\bigg|\frac{\partial u}{\partial x_j}\bigg|^2\bigg) dx} \sqrt{\int_\Omega\bigg(\sum_{j=1}^{d}\bigg|\frac{\partial v}{\partial x_j}\bigg|^2\bigg) dx}\\
&= \sqrt{\int_\Omega\big| \triangledown u \big|^2 dx} \sqrt{\int_\Omega\big| \triangledown v \big|^2 dx}\\
\end{aligned}
\end{equation}
\begin{equation}
\therefore \bigg| \int_{\Omega} \triangledown u \cdot \triangledown v dx \bigg| \leq \sqrt{\int_\Omega\big| \triangledown u \big|^2 dx} \sqrt{\int_\Omega\big| \triangledown v \big|^2 dx}
\end{equation}
\subsection{Energy (Revisited)}
\begin{equation}
E(u) := \frac{1}{2}\int_\Omega \sigma[u]:e[u]dx -\int_\Omega f\cdot u dx -\int_{\Gamma_N} q\cdot u ds
\end{equation}
with $u$ is a vector of the elasticity problem define by:
\begin{equation}\nonumber
\begin{aligned}
u\in\Hspace^1(\Omega:\R^d) &:= \{ u:\Omega \rightarrow\R^d |u=(u_i, \cdots, u_d), u_i\in\Hspace^1(\Omega) \}\\
&\Rightarrow E(u) < \infty
\end{aligned}
\end{equation}
$u:$ become solution $\Leftrightarrow u = argmin_{v\in\Hspace^1(\Omega:\R^d)}E(v)$
such a technique we call it variational principle.
\subsection{Variational Principle}
Let's consider a Poisson Equation Problem:
\begin{equation}\label{poissoneq}
\Omega \subset \R^d \begin{cases}
-\triangle u &= f(x) \in\Omega\\
u &= g(x) \text{ on } \Gamma_D\\
\frac{\partial u}{\partial v} &= q(x) \text{ on } \Gamma_N
\end{cases}
f\in L^2(\Omega), g\in H^1(\Omega), q\in L^2(\Gamma_N)
\end{equation}
\begin{remark}
	\begin{equation}\nonumber
	v \in H^1(\Omega) \Rightarrow \exists v|_\Gamma \in L^2(\Gamma)
	\end{equation}
	we choose $v \text{ on } L^2 \text{ because it will has value on the boundary }$
\end{remark}
\subsubsection{Definition of Weak Solution}
\begin{equation}\nonumber
u \in H^1(\Omega)\text{ s.t. } \begin{cases}
\int_\Omega \triangle u \cdot \triangle v dx = \int_\Omega fv dx + \int_{\Gamma_N} qv ds\\
\bigg(\forall v \in V := {v \in H^1(\Omega)\big| v|_{\Gamma_D}}\bigg)\\
v|_{\Gamma_D} = g|_{\Gamma_D} (v-g\in V)
\end{cases}
\end{equation}
$(v-g\in V)$ mean $(v\in V+g:={v+g|v\in V})$ with $V$ is an affine space.
\subsubsection{Definition of Strong Solution}
$u \in H^2(\Omega)$ and $u$ satisfies \eqref{poissoneq}
\begin{remark}
	\begin{equation}\nonumber
	\begin{aligned}
	H^2(\Omega):= \{ u\in L^2(\Omega) \frac{\partial u}{\partial x_j},\frac{\partial^2 u}{\partial x_i x_j} \in L^2(\Omega)\}\\
	u \in H^2(\Omega) \Rightarrow \frac{\partial u}{\partial x_j} \in H^1(\Omega)\\
	\frac{\partial u}{\partial}
	\end{aligned}
	\end{equation}
\end{remark}
\end{document}
