\documentclass[a4paper,12pt]{article}
\usepackage[a4paper, hmargin={1.5cm,1.5cm}, vmargin={1.5cm,1.5cm}]{geometry}
\usepackage{amsmath}
\usepackage{amsthm}
\usepackage{amsfonts}
\usepackage{color}
\usepackage[final]{graphicx}
\usepackage{subcaption}
\usepackage{wrapfig}
\newtheorem{remark}{Remark}[]
\newtheorem{prop}{Proposition}
\newtheorem{theorem}{Theorem}
\usepackage{amssymb}

\newcommand{\R}{\mathbb{R}}
\newcommand{\C}{\mathbb{C}}
\newcommand{\N}{\mathbb{N}}
\newcommand{\Q}{\mathbb{Q}}
\newcommand{\Lagr}{\mathcal{L}}


% Title Page
\title{Applied Analysis Report \\ Gronwall's Inequality}
\author{Alifian Mahardhika Maulana}


\begin{document}
\maketitle
\begin{enumerate}
	\item Prove the discrete Gronwall Inequality
		\begin{theorem} Discrete Gronwall Inequality\\
			Let $\{x^n\}_{n\geq 0},\{y^n\}_{n\geq 1},\{z^n\}_{n\geq 1},a>0,\triangle t: \text{small}\,\big( \triangle t \leq \frac{1}{2a} \big)$ be non-negative sequences, $T>0, N_T\leqq \big[ \frac{T}{\triangle t} \big]$
			\begin{equation}\label{eq:1}
			\frac{x^n - x^{n-1}}{\triangle t} + y^n \leq ax^n + z^n; \quad n\geq 1
			\end{equation}
			$\Rightarrow \exists c > 0$ independent of $\triangle t$ s.t.
			\begin{equation}\label{eq:2}
			\max_{n=0,\cdots,N_T} x^n + \triangle t \sum_{n=1}^{N_T}y^n \leq c\bigg(x^0 + \triangle t \sum_{n=1}^{N_T} z^n\bigg)
			\end{equation}
		\end{theorem}
	\textbf{Answer:}
	\begin{proof}
		We multiplied \eqref{eq:1} by $\triangle t$ we get:
		\begin{equation}\label{eq:3}
		x^n - x^{n-1}+ \triangle t y^n \leq a \triangle t x^n + \triangle t z^n
		\end{equation}
		take summation over $N_T$ for \eqref{eq:3} as follows:
		\begin{equation}\label{eq:4}
		\sum_{n=1}^{N_T}x^n - \sum_{n=1}^{N_T}x^{n-1}+ \triangle t \sum_{n=1}^{N_T}y^n \leq a \triangle t \sum_{n=1}^{N_T}x^n + \triangle t \sum_{n=1}^{N_T}z^n
		\end{equation}
		from \eqref{eq:4} we know that $x^n$ and $x^{n-1}$ in the left hand side cancelled out one and each other except for the first and last part, so \eqref{eq:4} becomes:
		\begin{equation}\label{eq:5}
		\begin{aligned}
		x^{N_T} -x^0 + \triangle t \sum_{n=1}^{N_T}y^n &\leq a \triangle t \sum_{n=1}^{N_T}x^n + \triangle t \sum_{n=1}^{N_T}z^n\\
		x^{N_T} + \triangle t \sum_{n=1}^{N_T}y^n &\leq x^0 + a \triangle t \sum_{n=1}^{N_T}x^n + \triangle t \sum_{n=1}^{N_T}z^n\\
		x^{N_T} - a \triangle t \sum_{n=1}^{N_T}x^n + \triangle t \sum_{n=1}^{N_T}y^n &\leq x^0 + \triangle t \sum_{n=1}^{N_T}z^n\\
		\end{aligned}
		\end{equation}
		\newpage
		then, for $a>0,\triangle t: \text{small}\,\big( \triangle t \leq \frac{1}{2a} \big), T>0, N_T\leqq \big[ \frac{T}{\triangle t} \big]$ and $x^n, y^n, z^n$ are a non-negative sequences,
		\iffalse
		\begin{equation}\label{eq:6}
		x^{N_T} - a \triangle t \sum_{n=1}^{N_T}x^n \leq \max_{n=0,\cdots,N_T} x^n
		\end{equation}
		We will proof \eqref{eq:6} below,
		\fi
		we define,
		$$A := \frac{x^{N_T} - a \triangle t \sum_{n=1}^{N_T}x^n + \triangle t \sum_{n=1}^{N_T}y^n}{x^0 + \triangle t \sum_{n=1}^{N_T}z^n}$$
		$$B := \frac{\max_{n=0,\cdots,N_T} x^n + \triangle t \sum_{n=1}^{N_T}y^n}{x^0 + \triangle t \sum_{n=1}^{N_T}z^n}$$
		First, take a condition where $A \geq B$, then,
		\begin{align*}
		\frac{\max_{n=0,\cdots,N_T} x^n + \triangle t \sum_{n=1}^{N_T}y^n}{x^0 + \triangle t \sum_{n=1}^{N_T}z^n} &\leq \max_{n=0,\cdots,N_T} x^n + N_T \triangle t \max_{n=0,\cdots,N_T} y^n\\
		&\leq \max_{n=0,\cdots,N_T} x^n + T y^n = c
		\end{align*}
		Second, take a condition where $A < B$, it is clear that
		\begin{align*}
		\frac{\max_{n=0,\cdots,N_T} x^n + \triangle t \sum_{n=1}^{N_T}y^n}{x^0 + \triangle t \sum_{n=1}^{N_T}z^n} \leq 1 = c
		\end{align*}
		then, we can find $c=\max\{1, \max_{n=0,\cdots,N_T} (x^n + T y^n)\}$ such that:
		\begin{equation}\label{eq:6}
		\max_{n=0,\cdots,N_T} x^n + \triangle t \sum_{n=1}^{N_T}y^n \leq c\bigg(x^0 + \triangle t \sum_{n=1}^{N_T} z^n\bigg)
		\end{equation}
	\end{proof}
\end{enumerate}
\end{document}