\documentclass[a4paper,12pt]{article}
\usepackage[a4paper, hmargin={1.5cm,1.5cm}, vmargin={2cm,2cm}]{geometry}
\usepackage{amsmath}
\usepackage{amsthm}
\usepackage{amsfonts}
\usepackage{color}
\usepackage[final]{graphicx}
\usepackage{subcaption}
\usepackage{wrapfig}
\newtheorem{remark}{Remark}[]
\newtheorem{prop}{Proposition}
\newtheorem{theorem}{Theorem}
\usepackage{amssymb}

\newcommand{\R}{\mathbb{R}}
\newcommand{\C}{\mathbb{C}}
\newcommand{\N}{\mathbb{N}}
\newcommand{\Q}{\mathbb{Q}}
\newcommand{\W}{\mathbb{W}}
\newcommand{\Vspace}{\mathbb{V}}
\newcommand{\Hspace}{\mathbb{H}}
\newcommand{\Lspace}{\mathbb{L}}
\newcommand{\Lagr}{\mathcal{L}}


% Title Page
\title{Assignment 3\\ Topics of Mathematical Science}
\author{Alifian Mahardhika Maulana}


\begin{document}
\maketitle
\begin{enumerate}
	\item Prove by Cauchy's Product formula that:
	\begin{equation}
	e^{z+w} = e^z e^w,\quad \forall z,w \in \C
	\end{equation}
	\textbf{Answer}:
	\begin{theorem}Cauchy Product Rule\\
		Let's consider these power series:
		$\sum\limits_{i=0}^{\infty}a_i x_i$ and $\sum\limits_{j=0}^{\infty}b_j x_j$
		With ${a_i}$ and ${b_j}$ be a complex coefficient. The Cauchy product of these power series are as follows:
		\begin{equation}
		\bigg( \sum\limits_{i=0}^{\infty}a_i x_i \bigg) \cdot \bigg( \sum\limits_{j=0}^{\infty}b_j x_j \bigg) = \sum\limits_{k=0}^{\infty} \sum\limits_{l=0}^{k} (a_l b_{k-l})x^k
		\end{equation}
	\end{theorem}
	then, we define $e^z$ and $e^w$ in form of Formal Power Series:
	\begin{align}\label{eq:ez}
	e^z = \sum\limits_{i=0}^{\infty} \frac{z^i}{i!}  \quad	e^w = \sum\limits_{j=0}^{\infty} \frac{w^j}{j!}
	\end{align}
	hence, the cauchy product of \eqref{eq:ez} are:
	\begin{equation}\label{eq:proof1}
	\begin{aligned}
	e^ze^w = \bigg( \sum\limits_{i=0}^{\infty} \frac{z^i}{i!} \bigg)	\cdot \bigg( \sum\limits_{j=0}^{\infty} \frac{w^j}{j!} \bigg) &= \sum\limits_{n=0}^{\infty}\sum\limits_{i=0}^{n} \frac{z^i}{i!} \frac{y^{n-i}}{(n-i)!} \\
	& = \sum\limits_{n=0}^{\infty}\frac{1}{n!} \sum\limits_{i=0}^{n} \begin{pmatrix}
	n\\
	i
	\end{pmatrix} z^i w^{n-1} = \sum\limits_{n=0}^{\infty}\frac{(z+w)^n}{n!} = e^{z+w}
	\end{aligned}
	\end{equation}
	\newpage
	\item Prove:\\
	Suppose FPS:
	\begin{equation}\label{eq:fz}
	f(z) = \sum_{n=0}^{\infty} a_n(z-z_0)^n
	\end{equation}
	converges absolutely on any compact set on ${|z-z_0|<R}$. Then \eqref{eq:fz} is complex differentiable on ${|z-z_0|<R}$ and $f'(z) = \sum_{n=1}^{\infty} n a_n(z-z_0)^{n-1}$\\
	\newline
	\textbf{Answer}:
	\eqref{eq:fz} is complex differentiable at $z$ if the limit
	\begin{equation}\label{eq:df}
	\lim_{h\to 0}\frac{f(z+h) - f(z)}{h}
	\end{equation} exist. This limit is denoted by $f'(z)$ or $\frac{df}{dz}$ Then, we calculate $f'(z)$ of \eqref{eq:fz} as follows:
	\begin{equation}
	\begin{aligned}
	f'(z) = \lim_{h\to 0}\frac{f(z+h) - f(z)}{h} &= \lim_{h\to 0}\frac{\sum_{n=0}^{\infty} a_n(z+h-z_0)^n - \sum_{n=0}^{\infty} a_n(z-z_0)^n}{h}\\
	&= \lim_{h\to 0}\sum_{n=0}^{\infty} a_n\frac{(z+h-z_0)^n - (z-z_0)^n}{h}\\
	&= \lim_{h\to 0}\sum_{n=0}^{\infty} a_n\frac{(z-z_0)^n + \sum_{k=1}^{n}\begin{pmatrix}
		n\\
		k
		\end{pmatrix}(z-z_0)^{n-1}h^k}{h}\\
	&= \sum_{n=0}^{\infty} a_n\lim_{h\to 0}\frac{hn(z-z_0)^{n-1} + h^2n((z-z_0)^{n-1} + \cdots)}{h}\\
	&= \sum_{n=0}^{\infty} a_n n(z-z_0)^{n-1} + \lim_{h\to 0}hn((z-z_0)^{n-1}) + \cdots\\
	&= \sum_{n=0}^{\infty} a_n n(z-z_0)^{n-1}\\
	\end{aligned}
	\end{equation}
\end{enumerate}
\end{document}